rustexamples/borrow_check_examples/unsupported_field_sensitive.rs
@@ -1,0 +1,10 @@
+// This program is not supported because of the limitation of the
+// reborrow mechanism (i.e., directly flowing the [p] to the region of y)
+// rustc +nightly unsupported_field_sensitive.rs -Z polonius=next
+fn main(){
+    let mut p = (12, 13);
+    let mut x = &mut p;
+    let mut y = &mut (*x).0;
+    p.1 = 15;
+    println!("{}", y);
+}
