rustexamples/test/borrow_test/11.rs
@@ -2,7 +2,7 @@ fn main(){
     let v: i32 = 1;
     let p: &mut i32 = &mut v;
     let q: &mut &mut i32 = &mut p;
-    v = 2;
+    v = 2; // invalidate the borrow of q; note that rustc reports error here
     let v1: i32 = 3;
-    *q = &mut v1;
+    *q = &mut v1; // cannot use q here; we report error here; what if we change mutable reference to immutable reference?
 }
