rustexamples/test/borrow_test/14.rs
@@ -3,8 +3,21 @@ fn main(){
     let tmp: i32 = 2;
     let p: &mut i32 = &mut v;
     let q: &mut i32 = &mut *p;
-    p = &mut tmp;
+    p = &mut tmp; // note that p is reassigned here
     *q = 5;
     v = 4;
-    *p = 3;
+    *p = 3; // using p does not affect v
 }
+
+// This example can be passed in Polonius, i.e., that our borrow checker is based on. But the NLL reports errors for these case
+
+// error[E0506]: cannot assign to `v` because it is borrowed
+//  --> src/main.rs:8:5
+//   |
+// 4 |     let mut p: &mut i32 = &mut v;
+//   |                           ------ `v` is borrowed here
+// ...
+// 8 |     v = 4;
+//   |     ^^^^^ `v` is assigned to here but it was already borrowed
+// 9 |     *p = 3;
+//   |     ------ borrow later used here
