rustexamples/test/borrow_test/16.rs
@@ -14,3 +14,14 @@ fn main(){
     printf("%d", *p);
 
 }
+
+// error[E0506]: cannot assign to `v` because it is borrowed
+//   --> src/main.rs:13:5
+//    |
+// 8  |         p = &mut v;
+//    |             ------ `v` is borrowed here
+// ...
+// 13 |     v = 4;
+//    |     ^^^^^ `v` is assigned to here but it was already borrowed
+// 14 |     println!("{}", *p);
+//    |                    -- borrow later used here
