rustexamples/test/borrow_test/18.rs
@@ -1,6 +1,6 @@
 fn main(){
     let a: Box<i32> = Box(1);
     let p: &mut i32 = &mut *a;
-    a = Box(2);
-    printf("%d", *p);
+    a = Box(2); //reassingment here which would invalidate p
+    printf("%d", *p); // report error here
 }
