rustexamples/test/borrow_test/28.rs
@@ -1,0 +1,104 @@
+// Current Polonius
+let mut v: i32 = 1;
+let p: &'p mut i32 = &'v mut v;
+v = 2; // Current Polonius reports error here: 
+       // 'p is live origin computed by liveness analysis, 
+       // so v is a live loan and accessing v is invalid
+... // unrelated code
+*p = 3;
+
+// Pure forward propagation
+let mut v: i32 = 1;
+let p: &'p mut i32 = &'v mut v;
+v = 2; // no error report here; accessing v would invalidate the origin 'p as {v} ⊆ 'p
+... // unrelated code
+*p = 3; // In pure forward propagation: 
+        // the error is reported here because using *p would access invalid origin 'p
+
+
+fn main(){
+    let mut v1: i32 = 1;
+    let mut v2: i32 = 2;
+    let mut p1: & 'p1 mut i32 = & 'v1 mut v1; 
+        // 'p1: {v1}
+    let mut p2: & 'p2 mut i32 = & 's_p1 mut *p1; 
+        // 'p1: {v1}, 'p2: {*p1, v1}
+    p1 = &'v2 mut v2; // 'p1: {v2}, 'p2: {v1}
+    *p1 = 3; // 'p1: {}, 'p2: {v1}
+    *p2 = 4; // 'p1: {}, 'p2: {v1}
+
+    v2 = 5; // 'p1: {}, 'p2: {v1}
+
+    v1 = 6; // 'p1: {}, 'p2: {v1}
+    println!("{}", *p2); // 'p1: {}, 'p2: {v1}
+}
+
+fn main(){
+    let mut v1: i32 = 1;
+    let mut v2: i32 = 2;
+    let mut p1: & 'p1 mut i32 = & 'v1 mut v1; 
+        // after this point: live loans is {v1}
+    let mut p2: & 'p2 mut i32 = & 's_p1 mut *p1; 
+        // live loans is {v1, *p1}
+    p1 = &'v2 mut v2; // {v1, v2}
+    *p1 = 3; // {v1}
+    *p2 = 4; // {v1}
+
+    v2 = 5; // {v1}
+
+    v1 = 6; 
+        // {v1}: Error! we use v1 but v1 is in the set of live loans!
+    println!("{}", *p2); // {}
+}
+
+// The syntax is not supported in our compiler
+// rustc +nightly -Z polonius 28.rs
+fn main(){
+    let mut v1: i32 = 1;
+    let mut v2: i32 = 2;
+    let mut p1: & 'p1 mut i32 = & 'v1 mut v1; 
+        // {v1} ⊆ 'v1, 'v1 ⊆ 'p1
+    let mut p2: & 'p2 mut i32 = & 's_p1 mut *p1; 
+        // {*p1} ⊆ 's_p1, 'p1 ⊆ 's_p1, 's_p1 ⊆ 'p2
+    p1 = &'v2 mut v2; // {v2} ⊆ 'v2, 'v2 ⊆ 'p1
+    *p1 = 3;
+    *p2 = 4;
+
+    v2 = 5;
+
+    v1 = 6;
+    println!("{}", *p2);
+}
+
+
+fn main(){
+    let mut v1: i32 = 1;
+    let mut v2: i32 = 2;
+    let mut p1: &mut i32 = &mut v1;
+    let mut p2: &mut i32 = &mut *p1;
+    p1 = &mut v2;
+    *p1 = 3;
+    *p2 = 4;
+
+    v2 = 5;
+
+    v1 = 6;
+    println!("{}", *p2);
+}
+
+fn main(){
+    let mut v1: i32 = 1;
+    let mut v2: i32 = 2;
+    let mut p1: & 'p1 mut i32 = & 'v1 mut v1; 
+        // after this point: live loans is {v1}
+    let mut p2: & 'p2 mut i32 = & 's_p1 mut *p1; 
+        // live loans is {v1, *p1}
+    p1 = &'v2 mut v2; // {v1, v2}
+    *p1 = 3; // {v1}
+    *p2 = 4; // {v1}
+
+    v2 = 5; // {v1}
+
+    v1 = 6; // {v1}
+    println!("{}", *p2); // {}
+}
