rustexamples/test/borrow_test/29.rs
@@ -1,0 +1,6 @@
+fn main(){
+    let b: Box<i32> = Box(1);
+    let a: Box<i32> = b;
+    let p: &mut Box<i32> = &mut b;
+    printf("p is %d", *p);
+}
