rustexamples/test/borrow_test/30.rs
@@ -1,0 +1,39 @@
+
+fn read_non_empty<'c>(x: &'c mut i32) -> &'c mut i32
+{
+    // 'c: {'c} 
+    // loop {
+    //     let b = &mut *x; // although mutable reference of *x would invalid 'b, reassigning b would make it valid again; 'b: {*x, 'c}
+    //     if *b > 3 {
+    //         return b; // 'c : {'c, *x}
+    //     } // 'c: {'c}
+    // }
+
+    
+    // let b = &mut *x; // although mutable reference of *x would invalid 'b, reassigning b would make it valid again; 'b: {*x, 'c}
+    // if *b > 3 {
+    //     return b; // 'c : {'c, *x}
+    // } // 'c: {'c}
+    
+    // b = &mut *x; // although mutable reference of *x would invalid 'b, reassigning b would make it valid again; 'b: {*x, 'c}
+    // if *b > 3 {
+    //     return b; // 'c : {'c, *x}
+    // } // 'c: {'c}
+    // return b;
+
+    let mut b: &mut i32 = &mut *x; // although mutable reference of *x would invalid 'b, reassigning b would make it valid again; 'b: {*x, 'c}
+    if *b > 3 {
+        return b; // 'c : {'c, *x}
+    } // 'c: {'c}
+    
+    b = &mut *x; // although mutable reference of *x would invalid 'b, reassigning b would make it valid again; 'b: {*x, 'c}
+    if *b > 3 {
+        return b; // 'c : {'c, *x}
+    } // 'c: {'c}
+    return b;
+}
+
+fn main(){
+    
+}
+//rustc +nightly 30.rs -Z dump-mir=all -Z polonius=next
