rustexamples/test/borrow_test/31.rs
@@ -1,0 +1,21 @@
+fn main(){
+    let mut v = 12;
+    let mut dummy1 = 13;
+    let mut dummy2 = 13;
+    let mut dummy_q1 = &mut dummy1;
+    let mut dummy_q2 = &mut dummy2;
+    let mut p = &mut v;
+    let mut q1 = &mut dummy_q1;
+    let mut q2 = &mut dummy_q2;
+    if true {
+        q1 = &mut p;
+    } else {
+        q2 = &mut p;
+    }
+    **q1 = 15;
+    **q2 = 20;
+    **q1 = 15;
+}
+// The borrow checker can judge that **q1 and **q2 are not aliased， but their regions are invariant?
+
+//rustc +nightly 31.rs -Z polonius=next
