rustexamples/test/borrow_test/32.rs
@@ -1,0 +1,36 @@
+//rustc +nightly 32.rs -Z polonius=next
+
+// fn cond() -> bool {
+//     return true;
+// }
+
+// fn unrelated() {
+//     let mut n = 1;
+//     while n < 100 {
+//         n += 1;
+//     }
+// }
+
+fn main(){
+    let v1 : i32 = 22;
+    let v2 : i32 = 44;
+    let p2: &mut i32 = &mut v2; // 'p2 -> {v2}
+    let p1: &mut i32 = &mut v1; // 'p1 -> {v1}, 'p2 -> {v2}
+    let q1: &mut &mut i32 = &mut p1; // 'q1 -> {p1}, ['p1, 'q2] -> {v1}, 'p2 -> {v2}
+    if true {
+        *p1 = 3; // 'q1 -> Invalid, ['p1, 'q2] -> {v1}, 'p2 -> {v2}
+        // p2 = &mut v2; // we cannot put p2 early because &mut v2 in the else branch would invalidate p2
+        q1 = &mut p2; // 'q1 -> {p2}, ['q2, 'p2] -> {v2}, 'p1 -> {v1}
+    } else {
+        *q1 = &mut *p2; // 'q1 -> {p1}, ['p1, 'q2] -> {v1, v2, *p2}, 'p2 -> {v2}
+        // v1 = 13;
+        // *p1 = 5;
+    } // 'q1 -> {p1, p2}, ['p1, 'p2, 'q2] -> {v1, v2, *p2}
+    v1 = 13; // 'q1 -> {p1, p2}, ['p1, 'p2, 'q2] -> Invalid
+             // After this line, using places containing one of 'p1, 'p2 and 'q2 would cause error
+    // *p1 = 3;
+    *p2 = 3;
+     **q1 = 5;
+    *p2 = 5; // error
+    **q1 = 3; // error
+}
