rustexamples/test/borrow_test/33.rs
@@ -1,0 +1,18 @@
+fn main(){
+    let v1: i32 = 22;
+    let v2: i32 = 44;
+    let p2: &mut i32 = &mut v2; // 'p2 -> {v2}
+    let p1: &mut i32 = &mut v1; // 'p1 -> {v1}, 'p2 -> {v2}
+    let q: &mut &mut i32;
+    if true {
+        q = &mut p1;
+    } else{
+        q = &mut p2;
+    } // 'q1 -> {p1, p2}, ['p1, 'p2, 'q2] -> {v1, v2}
+    **q = 3; // The following three lines are used to make sure that ‘q1, 'q2, 'p1 and 'p2 are all live before the end of the if-then-else, so that their invariant relations are merged at line 11
+    *p2 = 3;
+    *p1 = 2; // note that if we comment line 12, there is no error reported, because the relations betweem ('p1, 'q2) and ('p2, 'q2) are not merged
+    v1 = 13; // Using v1 should not invalidate p2 as it is impossible that p2 points to v1
+             // 'q1 -> {p1, p2}, ['p1, 'p2, 'q2] -> Invalid
+    *p2 = 3;
+}
