rustfrontend/PrintRustlight.ml
@@ -16,12 +16,12 @@ let temp_name (id: AST.ident) =
 
 let rec print_place out (p: place) =
   match p with
-  | Plocal(id, _) ->
-    fprintf out "%s" (extern_atom id)
-  | Pderef(p', _) ->
-    fprintf out "*%a " print_place p'
-  | Pfield(p', fid, _) ->
-    fprintf out "%a.%s" print_place p' (extern_atom fid)
+  | Plocal(id, ty) ->
+    fprintf out "%s with %s" (extern_atom id) (name_rust_type ty)
+  | Pderef(p', ty) ->
+    fprintf out "*%a with %s" print_place p' (name_rust_type ty)
+  | Pfield(p', fid, ty) ->
+    fprintf out "%a.%s with %s" print_place p' (extern_atom fid)  (name_rust_type ty)
   | Pdowncast(p',fid, _) ->
       fprintf out "(%a as %s)" print_place p' (extern_atom fid)
 
